src/HOL/Word/More_Word.thy
@@ -1,4 +1,4 @@
-(*  Title:      HOL/Word/More_Word.thy
+(*  Title:      HOL/Word/More_thy
 *)
 
 section \<open>Ancient comprehensive Word Library\<close>
@@ -14,5 +14,30 @@ imports
 begin
 
 declare signed_take_bit_Suc [simp]
+
+lemmas bshiftr1_def = bshiftr1_eq
+lemmas is_down_def = is_down_eq
+lemmas is_up_def = is_up_eq
+lemmas mask_def = mask_eq_decr_exp
+lemmas scast_def = scast_eq
+lemmas shiftl1_def = shiftl1_eq
+lemmas shiftr1_def = shiftr1_eq
+lemmas sshiftr1_def = sshiftr1_eq
+lemmas sshiftr_def = sshiftr_eq
+lemmas to_bl_def = to_bl_eq
+lemmas ucast_def = ucast_eq
+lemmas unat_def = unat_eq_nat_uint
+lemmas word_cat_def = word_cat_eq
+lemmas word_reverse_def = word_reverse_eq_of_bl_rev_to_bl
+lemmas word_roti_def = word_roti_eq_word_rotr_word_rotl
+lemmas word_rotl_def = word_rotl_eq
+lemmas word_rotr_def = word_rotr_eq
+lemmas word_sle_def = word_sle_eq
+lemmas word_sless_def = word_sless_eq
+
+lemma shiftl_transfer [transfer_rule]:
+  includes lifting_syntax
+  shows "(pcr_word ===> (=) ===> pcr_word) (<<) (<<)"
+  by (auto intro!: rel_funI word_eqI simp add: word.pcr_cr_eq cr_word_def word_size nth_shiftl)
 
 end
